WIP on TreeDEM interop tests

fstar/new/Test_Reader.ml
@@ -1,13 +1,28 @@
 open Test_Types
 
+let pow2 (x:int): int =
+  Z.to_int (Prims.pow2 (Z.of_int 32))
+
+let int_to_uint16 (x:int): FStar_UInt16.t =
+  if 0 <= x && x < pow2 16 then
+    FStar_UInt16.uint_to_t (Z.of_int x)
+  else
+    failwith "int_to_uint32: number of out bounds"
+
+let int_to_uint32 (x:int): FStar_UInt32.t =
+  if 0 <= x && x < pow2 32 then
+    FStar_UInt32.uint_to_t (Z.of_int x)
+  else
+    failwith "int_to_uint32: number of out bounds"
+
 let parse_uint32 (json:Yojson.Safe.t): FStar_UInt32.t =
   match json with
-  | `Int x -> (FStar_UInt32.uint_to_t (Z.of_int x))
+  | `Int x -> int_to_uint32 x
   | _ -> failwith "parse_uint32: not an int"
 
 let parse_optional_uint32 (json:Yojson.Safe.t): FStar_UInt32.t option =
   match json with
-  | `Int x -> Some (FStar_UInt32.uint_to_t (Z.of_int x))
+  | `Int x -> Some (int_to_uint32 x)
   | `Null -> None
   | _ -> failwith "parse_optional_uint32: not an int or null"
 
@@ -15,8 +30,8 @@ let parse_treemath_test (json:Yojson.Safe.t): treemath_test =
   match json with
   | `Assoc [("n_leaves", `Int n_leaves); ("n_nodes", `Int n_nodes); ("root", `List root); ("left", `List left); ("right", `List right); ("parent", `List parent); ("sibling", `List sibling)] ->
     ({
-      n_leaves=FStar_UInt32.uint_to_t (Z.of_int n_leaves);
-      n_nodes=FStar_UInt32.uint_to_t (Z.of_int n_nodes);
+      n_leaves=int_to_uint32 n_leaves;
+      n_nodes=int_to_uint32 n_nodes;
       root=List.map parse_uint32 root;
       left=List.map parse_optional_uint32 left;
       right=List.map parse_optional_uint32 right;
@@ -25,9 +40,65 @@ let parse_treemath_test (json:Yojson.Safe.t): treemath_test =
     })
   | _ -> failwith "parse_treemath_test: incorrect test vector format"
 
+let parse_keyschedule_test_epoch (json:Yojson.Safe.t): keyschedule_test_epoch_input * keyschedule_test_epoch_output =
+  match json with
+  | `Assoc [
+    ("tree_hash", `String tree_hash);
+    ("commit_secret", `String commit_secret);
+    ("psk_secret", `String psk_secret);
+    ("confirmed_transcript_hash", `String confirmed_transcript_hash);
+    ("group_context", `String group_context);
+    ("joiner_secret", `String joiner_secret);
+    ("welcome_secret", `String welcome_secret);
+    ("init_secret", `String init_secret);
+    ("sender_data_secret", `String sender_data_secret);
+    ("encryption_secret", `String encryption_secret);
+    ("exporter_secret", `String exporter_secret);
+    ("authentication_secret", `String authentication_secret);
+    ("external_secret", `String external_secret);
+    ("confirmation_key", `String confirmation_key);
+    ("membership_key", `String membership_key);
+    ("resumption_secret", `String resumption_secret);
+    ("external_pub", `String external_pub)
+  ] ->
+    ({
+      tree_hash = tree_hash;
+      commit_secret = commit_secret;
+      psk_secret = psk_secret;
+      confirmed_transcript_hash = confirmed_transcript_hash;
+    }, {
+      group_context = group_context;
+      joiner_secret = joiner_secret;
+      welcome_secret = welcome_secret;
+      init_secret = init_secret;
+      sender_data_secret = sender_data_secret;
+      encryption_secret = encryption_secret;
+      exporter_secret = exporter_secret;
+      authentication_secret = authentication_secret;
+      external_secret = external_secret;
+      confirmation_key = confirmation_key;
+      membership_key = membership_key;
+      resumption_secret = resumption_secret;
+      external_pub = external_pub;
+    })
+  | _ -> failwith "parse_keyschedule_test_epoch: incorrect test vector format"
+
+
+let parse_keyschedule_test (json:Yojson.Safe.t): keyschedule_test =
+  match json with
+  | `Assoc [("cipher_suite", `Int cipher_suite); ("group_id", `String group_id); ("initial_init_secret", `String initial_init_secret); ("epochs", `List epochs)] ->
+    {
+      cipher_suite = int_to_uint16 cipher_suite;
+      group_id = group_id;
+      initial_init_secret = initial_init_secret;
+      epochs = List.map parse_keyschedule_test_epoch epochs;
+    }
+  | _ -> failwith "parse_keyschedule_test: incorrect test vector format"
+
 let get_filename (typ:test_type): string =
   match typ with
   | TreeMath -> "test_vectors/treemath.json"
+  | KeySchedule -> "test_vectors/key_schedule.json"
 
 let get_testsuite (typ:test_type): testsuite =
   let json = Yojson.Safe.from_channel (open_in (get_filename typ)) in
@@ -36,5 +107,11 @@ let get_testsuite (typ:test_type): testsuite =
     match json with
     | `List l ->
       (TreeMath_test (List.map parse_treemath_test l))
+    | _ -> failwith "get_testsuite: incorrect test vector format"
+  end
+  | KeySchedule -> begin
+    match json with
+    | `List l ->
+      (KeySchedule_test (List.map parse_keyschedule_test l))
     | _ -> failwith "get_testsuite: incorrect test vector format"
   end
