fstar/new/Crypto.Derived.fst
@@ -1,10 +1,42 @@
-module CryptoMLS
+module Crypto.Derived
 
-include Crypto
-open Lib.Result
+friend Crypto.Builtins
+
 open Parser
+open NetworkTypes
 open Lib.IntTypes
-open Lib.ByteSequence
+
+module DH = Spec.Agile.DH
+module AEAD = Spec.Agile.AEAD
+module Hash = Spec.Agile.Hash
+
+let ciphersuite_from_nt cs =
+  match cs with
+  | CS_mls10_128_dhkemx25519_aes128gcm_sha256_ed25519 -> return ({
+    kem_dh = DH.DH_Curve25519;
+    kem_hash = Hash.SHA2_256;
+    aead = AEAD.AES128_GCM;
+    kdf_hash = Hash.SHA2_256;
+    signature = Ed_25519;
+  })
+  | CS_mls10_128_dhkemp256_aes128gcm_sha256_p256 -> return ({
+    kem_dh = DH.DH_P256;
+    kem_hash = admit();
+    aead = admit();
+    kdf_hash = admit();
+    signature = admit();
+  })
+  | CS_mls10_128_dhkemx25519_chacha20poly1305_sha256_ed25519 -> return ({
+    kem_dh = DH.DH_Curve25519;
+    kem_hash = Hash.SHA2_256;
+    aead = AEAD.CHACHA20_POLY1305;
+    kdf_hash = Hash.SHA2_256;
+    signature = Ed_25519;
+  })
+  | CS_mls10_256_dhkemx448_aes256gcm_sha512_ed448 -> fail "ciphersuite_from_nt: ciphersuite not available"
+  | CS_mls10_256_dhkemp521_aes256gcm_sha512_p521 -> fail "ciphersuite_from_nt: ciphersuite not available"
+  | CS_mls10_256_dhkemx448_chacha20poly1305_sha512_ed448 -> fail "ciphersuite_from_nt: ciphersuite not available"
+  | _ -> fail "ciphersuite_from_nt: bad ciphersuite"
 
 noeq type kdf_label_nt = {
   kln_length: uint16;
@@ -23,7 +55,6 @@ let ps_kdf_label =
     (fun (|length, (|label, context|)|) -> {kln_length=length; kln_label=label; kln_context=context;})
     (fun x -> (|x.kln_length, (|x.kln_label, x.kln_context|)|))
 
-val expand_with_label: ciphersuite -> secret:bytes -> label:bytes -> context:bytes -> len:size_nat -> result (lbytes len)
 let expand_with_label cs secret label context len =
   assert_norm (String.strlen "mls10 " == 6);
   if not (len < pow2 16) then
@@ -42,6 +73,5 @@ let expand_with_label cs secret label context len =
     }) in
     kdf_expand cs secret kdf_label len
 
-val derive_secret: cs:ciphersuite -> secret:bytes -> label:bytes -> result (lbytes (kdf_length cs))
 let derive_secret cs secret label =
   expand_with_label cs secret label bytes_empty (kdf_length cs)
