fstar/new/Crypto.Derived.fsti
@@ -1,0 +1,11 @@
+module Crypto.Derived
+
+open Crypto.Builtins
+open Lib.Result
+open Lib.IntTypes
+open Lib.ByteSequence
+open NetworkTypes
+
+val ciphersuite_from_nt: cipher_suite_nt -> result ciphersuite
+val expand_with_label: ciphersuite -> secret:bytes -> label:bytes -> context:bytes -> len:size_nat -> result (lbytes len)
+val derive_secret: cs:ciphersuite -> secret:bytes -> label:bytes -> result (lbytes (kdf_length cs))
