fstar/new/Test.Types.fst
@@ -1,9 +1,7 @@
 module Test.Types
 
 module U32 = FStar.UInt32
-
-type test_type =
-  | TreeMath
+module U16 = FStar.UInt16
 
 type treemath_test = {
   n_leaves: U32.t;
@@ -15,5 +13,43 @@ type treemath_test = {
   sibling: list (option U32.t);
 }
 
+type keyschedule_test_epoch_input = {
+  tree_hash: string;
+  commit_secret: string;
+  psk_secret: string;
+  confirmed_transcript_hash: string;
+}
+
+type keyschedule_test_epoch_output = {
+  group_context: string;
+
+  joiner_secret: string;
+  welcome_secret: string;
+  init_secret: string;
+
+  sender_data_secret: string;
+  encryption_secret: string;
+  exporter_secret: string;
+  authentication_secret: string;
+  external_secret: string;
+  confirmation_key: string;
+  membership_key: string;
+  resumption_secret: string;
+
+  external_pub: string;
+}
+
+type keyschedule_test = {
+  cipher_suite: U16.t;
+  group_id: string;
+  initial_init_secret: string;
+  epochs: list (keyschedule_test_epoch_input & keyschedule_test_epoch_output);
+}
+
+type test_type =
+  | TreeMath
+  | KeySchedule
+
 type testsuite =
   | TreeMath_test: list treemath_test -> testsuite
+  | KeySchedule_test: list keyschedule_test -> testsuite
