fstar/new/Test.fst
@@ -5,9 +5,10 @@ open FStar.All
 open Test.Types
 open Test.Reader
 open Test.TreeMath
+open Test.KeySchedule
 open Test.Utils
 
-let main =
+let run_treemath_tests =
   match get_testsuite TreeMath with
   | TreeMath_test l -> begin
     if test_treemath l then (
@@ -17,3 +18,18 @@ let main =
     )
   end
   | _ -> IO.print_string "TreeMath: got the wrong type of testsuite (internal error)\n"
+
+let run_keyschedule_tests =
+  match get_testsuite KeySchedule with
+  | KeySchedule_test l -> begin
+    if test_keyschedule l then (
+      IO.print_string ("KeySchedule: success (" ^ (nat_to_string (List.Tot.length l)) ^ " tests)\n")
+    ) else (
+      IO.print_string "KeySchedule: failure\n"
+    )
+  end
+  | _ -> IO.print_string "KeySchedule: got the wrong type of testsuite (internal error)\n"
+
+let main =
+  run_treemath_tests;
+  run_keyschedule_tests
