fstar/new/Tree.fst
@@ -16,7 +16,7 @@ type path (l:nat) (n:tree_size l) (i:leaf_index n) (leaf_t:Type) (node_t:Type) =
 type direction = | Left | Right
 //let index_l (l:nat) = x:nat{x < pow2 l}
 
-let child_index (#n:nat) (l:pos{pow2 (l-1) < n}) (i:leaf_index n) : (dir:direction & (if dir = Left then leaf_index (pow2 (l-1)) else leaf_index (n-pow2 (l-1)))) =
+let child_index (#n:nat) (l:pos{pow2 (l-1) < n}) (i:leaf_index n) : (dir:direction & (leaf_index (if dir = Left then (pow2 (l-1)) else (n-pow2 (l-1))))) =
   if i < pow2 (l - 1) then (|Left, i|) else (|Right, i-pow2 (l-1)|)
 //let child_index (l:pos) (i:index_l l) : index_l (l-1) & direction =
 //  if i < pow2 (l - 1) then (i,Left) else (i-pow2 (l-1),Right)
